refactored relational examples, workaraund for some performance issues

examples/relational/sample_examples.fst
@@ -10,6 +10,7 @@ open Heap
 open Comp
 open Sample
 open Bijection
+open Relational
 
 let c0_pfx a = a := 0
 let c1_pfx b = b := 1
@@ -22,20 +23,24 @@ let equiv_sfx a b c d = compose2 c0_sfx c1_sfx (a, c) (b, d)
 let dec x = x - 1
 let inc x = x + 1
 
+val dec_good_sample : unit -> Lemma (good_sample_fun dec)
+let dec_good_sample () = cut(inverses dec inc);
+                         lemma_inverses_bij  dec inc ;
+                         bijection_good_sample_fun dec
+
+
 (* relate the programs
   c0_pfx ; sample ; c0_sfx  and
   c1_pfx ; sample ; c1_sfx  *)
 val equiv_seq: a:ref int
                -> b:ref int
-               -> ST2 (unit * unit)
+               -> ST2 (double unit)
                   (requires (fun _ -> True))
-                  (ensures (fun _ _ h2 -> sel (fst h2) a = sel (snd h2) b))
+                  (ensures (fun _ _ h2 -> sel (R.l h2) a = sel (R.r h2) b))
 let equiv_seq a b = let _ = equiv_pfx a b in
-                    cut (inverses dec inc);
-                    let c, d = sample (fun x -> dec x) in
+                    dec_good_sample ();
+                    let R c d = sample (fun x -> dec x) in
                     equiv_sfx a b c d
-
-
 
 (* Encryption with xor (Example from RF* paper) *)
 module Example2
@@ -43,28 +48,35 @@ open Heap
 open Comp
 open Sample
 open Bijection
+open Relational
 open Xor
 
 let encrypt p k = xor p k
 let decrypt c k = xor c k
 
+val cpa_good_sample_fun: a:block -> b:block ->
+  Lemma (good_sample_fun #block #block (fun x -> xor (xor a b) x))
+let cpa_good_sample_fun a b =
+  let sample_fun = (fun x -> xor (xor a b) x) in
+  cut (inverses #block #block sample_fun sample_fun);
+  lemma_inverses_bij #block #block sample_fun sample_fun;
+  bijection_good_sample_fun #block #block sample_fun
+
 val cpa : block
        -> block
-       -> ST2 (block * block)
+       -> ST2 (double block)
             (requires (fun _ -> True))
-            (ensures (fun _ p _ -> fst p = snd p))
+            (ensures (fun _ p _ -> R.l p = R.r p))
 let cpa a b = let sample_fun = (fun x -> xor (xor a b) x) in
-              cut (inverses #block #block sample_fun sample_fun);
-              let k1, k2 = sample sample_fun in
+              cpa_good_sample_fun a b;
+              let R k1 k2 = sample sample_fun in
               compose2 (fun k -> encrypt a k) (fun k -> encrypt b k) k1 k2
               (* This does not work with eta reduced versions of the function *)
 
 (* As this example does not use state, we actually don't need the ST2 monad *)
-val cpa' : block
-        -> block
-        -> Tot (r:(block * block){fst r = snd r})
-let cpa' a b = let sample_fun = (fun x -> xor (xor a b) x) in
-              cut (inverses #block #block sample_fun sample_fun);
-              let k1, k2 = sample sample_fun in
-              encrypt a k1, encrypt b k2
-              (* This does not work with eta reduced versions of the function *)
+val cpa' : double block
+        -> Tot (eq block)
+let cpa' b = let sample_fun = (fun x -> xor (xor (R.l b) (R.r b)) x) in
+              cpa_good_sample_fun (R.l b) (R.r b);
+              let k = sample sample_fun in
+              rel_map2 encrypt b k
