lib/st2.fst
@@ -3,9 +3,45 @@
     variables:LIB=../lib;
     other-files:$LIB/set.fsi $LIB/heap.fst $LIB/st.fst
   --*)
+
+module Relational
+open Heap
+type rel (a:Type) (b:Type) : Type =
+  | R : l:a -> r:b -> rel a b
+
+let twice x = R x  x
+type double (t:Type) = rel t  t
+type eq (t:Type) = p:(double t){R.l p = R.r p}
+
+
+val rel_map1 : ('a -> Tot 'b) -> (double 'a) -> Tot (double 'b)
+let rel_map1 f (R x1 x2)  = R (f x1) (f x2)
+
+val rel_map2 : ('a -> 'b -> Tot 'c) -> (double 'a) -> (double 'b) -> Tot (double 'c)
+let rel_map2 f (R x1 x2) (R y1 y2) = R (f x1 y1) (f x2 y2)
+
+val rel_map3 : ('a -> 'b -> 'c -> Tot 'd) -> (double 'a) -> (double 'b) -> (double 'c) -> Tot (double 'd)
+let rel_map3 f (R x1 x2) (R y1 y2) (R z1 z2) = R (f x1 y1 z1) (f x2 y2 z2)
+
+let add_rel (R a b) (R c d) = R (a+c) (b+d)
+let mul_rel (R a b) (R c d) = R (a*c) (b*d)
+val tl_rel: #a:Type -> l:double (list a){is_Cons (R.l l) /\ is_Cons (R.r l)}-> Tot (double (list a))
+let tl_rel (R (_::xs) (_::ys)) = R xs ys
+let cons_rel (R x y) (R xs ys) = R (x::xs)  (y::ys)
+let pair_rel (R x y) (R x' y') = R (x,x') (y,y')
+let fst_rel (R (x, y) (x', y')) = R x x'
+let snd_rel (R (x, y) (x', y')) = R y y'
+let and_rel (R a b) = a && b
+let or_rel (R a b) = a || b
+let eq_rel (R a b) = a = b
+let sel_rel (R h0 h1) (R r0 r1) = R (sel h0 r0) (sel h1 r1)
+
+
+
 module Comp
 open Heap
-type heap2 = heap * heap
+open Relational
+type heap2 = double heap
 
 new_effect STATE2 = STATE_h heap2
 kind ST2Pre = STPre_h heap2
@@ -18,11 +54,11 @@ effect St2 (a:Type) = ST2 a (fun h -> True) (fun h0 r h1 -> True)
 sub_effect
   PURE   ~> STATE2 = (fun (a:Type) (wp:PureWP a) (p:ST2Post a) -> (fun h2 -> wp (fun a0 -> p a0 h2)))
 
-type comp (a:Type) (b:Type) (wp0:STWP a) (wp1:STWP b) (p:((a * b) -> heap2 -> Type)) (h2:heap2) =
+type comp (a:Type) (b:Type) (wp0:STWP a) (wp1:STWP b) (p:((rel a b) -> heap2 -> Type)) (h2:heap2) =
     wp0 (fun y0 h0 ->
-      wp1 (fun y1 h1 -> p (y0, y1) (h0, h1))
-      (snd h2))
-    (fst h2)
+      wp1 (fun y1 h1 -> p (R y0 y1) (R h0 h1))
+      (R.r h2))
+    (R.l h2)
 
 assume val compose2: #a0:Type -> #b0:Type -> #wp0:(a0 -> STWP b0) -> #wlp0:(a0 -> STWP b0)
                   -> #a1:Type -> #b1:Type -> #wp1:(a1 -> STWP b1) -> #wlp1:(a1 -> STWP b1)
@@ -30,6 +66,6 @@ assume val compose2: #a0:Type -> #b0:Type -> #wp0:(a0 -> STWP b0) -> #wlp0:(a0 -
                   -> =c1:(x1:a1 -> STATE b1 (wp1 x1) (wlp1 x1))
                   -> x0:a0
                   -> x1:a1
-                  -> STATE2 (b0 * b1)
+                  -> STATE2 (rel b0 b1)
                              (comp b0 b1 (wp0 x0) (wp1 x1))
                              (comp b0 b1 (wlp0 x0) (wlp1 x1))
