examples/relational/noninterference.fst
@@ -8,20 +8,21 @@ module NonInterference
 
 open Comp
 open Heap
+open Relational
 
 assume val high : ref 'a -> Tot bool
 let low x = not (high x)
 
-type ni = unit -> 
-          ST2 (unit * unit)
-              (requires (fun h2 -> (forall (x:ref int). low x ==> 
-                                            sel (fst h2) x = sel (snd h2) x)))
-              (ensures  (fun _ _ h2 -> (forall (x:ref int). low x ==> 
-                                            sel (fst h2) x = sel (snd h2) x)))
+type ni = unit ->
+          ST2 (rel unit unit)
+              (requires (fun h2 -> (forall (x:ref int). low x ==>
+                                            sel (R.l h2) x = sel (R.r h2) x)))
+              (ensures  (fun _ _ h2 -> (forall (x:ref int). low x ==>
+                                            sel (R.l h2) x = sel (R.r h2) x)))
 
 assume val new_low : unit -> x:ref int{low x}
 assume val new_high : unit -> x:ref int{high x}
- 
+
 let a = new_low ()
 let b = new_high ()
 let c = new_high ()
@@ -29,9 +30,9 @@ let d = new_low ()
 
 let test1 () = (if !b = 0 then
                  a := 2
-               else 
-                 a := 1); 
+               else
+                 a := 1);
                a := 0
 
 val test1_ni : ni
-let test1_ni () = compose2 test1 test1 () () 
+let test1_ni () = compose2 test1 test1 () ()
