examples/relational/sample.fst
@@ -1,3 +1,9 @@
+(*--build-config
+    options:--admit_fsi Set --z3timeout 5;
+    variables:LIB=../../lib;
+    other-files:$LIB/set.fsi $LIB/heap.fst $LIB/st.fst $LIB/all.fst $LIB/st2.fst $LIB/bytes.fst
+  --*)
+
 module Bijection
 
 opaque type injection (#a:Type) (#b:Type) (f:a -> Tot b) = (forall (x:a) (y:a). f x = f y ==> x = y)
@@ -7,15 +13,25 @@ type bij (#a:Type) (#b:Type) = f:(a -> Tot b){bijection f}
 opaque type inverses (#a:Type) (#b:Type) (f:a -> Tot b) (g:b -> Tot a) =
    (forall (y:b). f (g y) = y) /\
    (forall (x:a). g (f x) = x)
-opaque val lemma_inverses_bij: a:Type -> b:Type -> f:(a -> Tot b) -> g:(b -> Tot a) ->
+opaque val lemma_inverses_bij: #a:Type -> #b:Type -> f:(a -> Tot b) -> g:(b -> Tot a) ->
   Lemma (requires (inverses f g))
         (ensures (bijection f))
 let lemma_inverses_bij f g = ()
 
+assume logic type good_sample_fun (#a:Type) (#b:Type) (f:a -> Tot b)
+assume val bijection_good_sample_fun : #a:Type -> #b:Type -> f:(a -> Tot b) ->
+  Lemma (requires (bijection f))
+        (ensures  (good_sample_fun f))
+assume val good_sample_fun_bijection : #a:Type -> #b:Type -> f:(a -> Tot b) ->
+  Lemma (requires (good_sample_fun f))
+        (ensures  (bijection f))
+
+
 module Sample
 open Bijection
+open Relational
 
 (* sample two random values such that they are related by a bijection f *)
 assume val sample : #a:Type -> #b:Type
-                    -> f:(a -> Tot b){bijection f}
-                    -> Tot (r:(a * b) {snd r = f (fst r)})
+                    -> f:(a -> Tot b){good_sample_fun f}
+                    -> Tot (r:(rel a  b) {R.r r = f (R.l r)})
